Started adding suppport for maps with key types other than uint64

src/goose_lang/lib/into_val.v
@@ -23,16 +23,17 @@ Qed.
 
 (* IntoVal where the value is guaranteed to be comparable, e.g. OK to use as the
    key type in a map *)
-Class IntoValComparable {ext} V {H: @IntoVal ext V} :=
+Class IntoValComparable V `{IntoVal V} :=
   {
-    IntoValComparable_fact (v:V): is_comparable (to_val v);
+    IntoValComparable_comparable (v:V): is_comparable (to_val v);
+    IntoValComparable_inj (v:V) (vval:val) : from_val vval = Some v → to_val v = vval
   }.
 
 #[global]
-Hint Mode IntoValComparable - ! - : typeclass_instances.
+Hint Mode IntoValComparable ! - - : typeclass_instances.
 
 (* IntoVal for a particular GooseLang type *)
-Class IntoValForType {ext} V {H: @IntoVal ext V} {ext_ty: ext_types ext} (t:ty) :=
+Class IntoValForType V {ext} {H: @IntoVal ext V} {ext_ty: ext_types ext} (t:ty) :=
     { def_is_zero: to_val (IntoVal_def V) = zero_val t;
       to_val_has_zero: has_zero t;
       (* TODO: this isn't necessary, but it seems reasonable *)
@@ -41,7 +42,7 @@ Class IntoValForType {ext} V {H: @IntoVal ext V} {ext_ty: ext_types ext} (t:ty) 
 #[global]
 Hint Mode IntoValForType - - - - ! : typeclass_instances.
 #[global]
-Hint Mode IntoValForType - ! - - - : typeclass_instances.
+Hint Mode IntoValForType ! - - - - : typeclass_instances.
 
 #[global]
 Instance Permutation_inj_list_fmap {A B} (f: A -> B) `{!Inj eq eq f} :
@@ -103,7 +104,13 @@ Section instances.
     constructor; auto.
   Qed.
   Global Instance u64_IntoValComparable : IntoValComparable u64.
-  Proof. by constructor. Qed.
+  Proof.
+    constructor; try done.
+    intros. simpl in *.
+    destruct vval; try done; destruct l; try done.
+    repeat f_equal.
+    by injection H.
+  Qed.
 
   Global Instance u8_IntoVal : IntoVal u8.
   Proof.
@@ -116,7 +123,13 @@ Section instances.
     constructor; eauto.
   Qed.
   Global Instance u8_IntoValComparable : IntoValComparable u8.
-  Proof. by constructor. Qed.
+  Proof.
+    constructor; try done.
+    intros. simpl in *.
+    destruct vval; try done; destruct l; try done.
+    repeat f_equal.
+    by injection H.
+  Qed.
 
   Global Instance loc_IntoVal : IntoVal loc.
   Proof.
@@ -137,7 +150,13 @@ Section instances.
     constructor; auto.
   Qed.
   Global Instance loc_IntoValComparable : IntoValComparable loc.
-  Proof. by constructor. Qed.
+  Proof.
+    constructor; try done.
+    intros. simpl in *.
+    destruct vval; try done; destruct l; try done.
+    repeat f_equal.
+    by injection H.
+  Qed.
 
   Global Instance slice_IntoVal : IntoVal Slice.t.
     refine
@@ -154,8 +173,23 @@ Section instances.
     apply slice_val_ty.
   Qed.
   Global Instance slice_IntoValComparable : IntoValComparable Slice.t.
-  Proof. by constructor. Qed.
-
+  Proof.
+    constructor; try done.
+    intros.
+    destruct vval; try done.
+    simpl in *.
+    destruct vval1; try done; destruct vval1_1; try done.
+    destruct l; try done.
+    destruct vval1_2; try done.
+    destruct l0; try done.
+    destruct vval2; try done.
+    destruct l0; try done.
+    destruct v.
+    injection H.
+    intros.
+    subst.
+    done.
+  Qed.
 
   Global Instance bool_IntoVal : IntoVal bool.
   Proof.
@@ -166,7 +200,13 @@ Section instances.
   Global Instance bool_IntoVal_boolT : IntoValForType bool boolT.
   Proof. constructor; auto. Qed.
   Global Instance bool_IntoValComparable : IntoValComparable bool.
-  Proof. by constructor. Qed.
+  Proof.
+    constructor; try done.
+    intros. simpl in *.
+    destruct vval; try done; destruct l; try done.
+    repeat f_equal.
+    by injection H.
+  Qed.
 
   Global Instance string_IntoVal : IntoVal string.
   Proof.
@@ -177,7 +217,13 @@ Section instances.
   Global Instance string_IntoVal_boolT : IntoValForType string stringT.
   Proof. constructor; auto. Qed.
   Global Instance string_IntoValComparable : IntoValComparable string.
-  Proof. by constructor. Qed.
+  Proof.
+    constructor; try done.
+    intros. simpl in *.
+    destruct vval; try done; destruct l; try done.
+    repeat f_equal.
+    by injection H.
+  Qed.
 
   Global Instance unit_IntoVal : IntoVal ().
   Proof.
@@ -190,6 +236,10 @@ Section instances.
   Global Instance unit_IntoValForType : IntoValForType () unitT.
   Proof. constructor; auto. Qed.
   Global Instance unit_IntoValComparable : IntoValComparable unit.
-  Proof. by constructor. Qed.
+  Proof.
+    constructor; try done.
+    intros. simpl in *.
+    destruct vval; try done; destruct l; try done.
+  Qed.
 
 End instances.
